src/Layer1to2Refinement.v
@@ -4,8 +4,8 @@ Require Import FunctionalExtensionality Omega.
 
 Section Layer1to2Refinement.
   
-  Fixpoint compile {T} (p1: Layer2.prog T) : Layer1.prog T :=
-    match p1 with
+  Fixpoint compile {T} (p2: Layer2.prog T) : Layer1.prog T :=
+    match p2 with
     | Read a => read a
     | Write a v => write a v
     | Alloc v => alloc v
@@ -13,131 +13,619 @@ Section Layer1to2Refinement.
     | Ret v => Layer1.Ret v
     | Bind px py => Layer1.Bind (compile px) (fun x => compile (py x))
     end.
+
   
-  Fixpoint oracle_matches T (d1: Layer1.state) (p: Layer2.prog T)  (o1: oracle Layer1.token) (o2: oracle Layer2.token) :=
+  Fixpoint oracle_refines_to T (d1: Layer1.state) (p: Layer2.prog T)  (o1: BaseTypes.oracle Layer1.token) (o2: Layer2.oracle) : Prop :=
     match p with
     | Alloc v =>
-      forall d1',
-        (Layer1.exec o1 d1 (compile (Alloc v)) (Crashed d1') ->
-         o2 = [Crash]) /\
-        (forall r, Layer1.exec o1 d1 (compile (Alloc v)) (Finished d1' r) ->
-         match r with
-         | Some a =>
-           o2 = [BlockNum a]
-         | None =>
-           o2 = [DiskFull]
-         end)
+      if (in_dec Layer1.token_dec Layer1.Crash o1) then
+        o2 = {| token_list := [Crash]; refinement_length := length o1 |}
+      else
+        let sv := Disk.read d1 0 in
+        match sv with
+        | Some v =>
+          let bits := bits (value_to_bits v) in
+          let index := get_first_zero bits in
+          
+          if lt_dec index block_size then
+            o2 = {| token_list := [BlockNum index]; refinement_length := length o1 |}
+          else
+            o2 = {| token_list := [DiskFull]; refinement_length := length o1 |}
+        | None => False
+        end
     | @Bind T1 T2 p1 p2 =>
-       forall d1',
-        (Layer1.exec o1 d1 (compile p1) (Crashed d1') ->
-         oracle_matches T1 d1 p1 o1 o2) /\
-        (forall r o1' o1'' o2' o2'',
-           o1 = o1'++o1'' ->
-           o2 = o2'++o2'' ->
-           Layer1.exec o1' d1 (compile p1) (Finished d1' r) ->
-           oracle_matches T1 d1 p1 o1' o2' /\
-           oracle_matches T2 d1' (p2 r) o1'' o2'')
+
+      exists d1',
+      (Layer1.exec o1 d1 (compile p1) (Crashed d1') /\
+         oracle_refines_to T1 d1 p1 o1 o2) \/
+      (exists r o1' o1'' o2' o2'' ret,
+         o1 = o1'++o1'' /\
+         Layer1.exec o1' d1 (compile p1) (Finished d1' r) /\
+         Layer1.exec o1'' d1' (compile (p2 r)) ret /\
+         oracle_refines_to T1 d1 p1 o1' o2' /\
+         oracle_refines_to T2 d1' (p2 r) o1'' o2'' /\
+         o2 = {| token_list:= token_list o2'++ token_list o2'';
+                 refinement_length := refinement_length o2' + refinement_length o2'' |})
     | _ =>
-      forall d1',
-        (Layer1.exec o1 d1 (compile p) (Crashed d1') ->
-         o2 = [Crash]) /\
-        (forall r, Layer1.exec o1 d1 (compile p) (Finished d1' r) ->
-         o2 = [Cont])
+      if (in_dec Layer1.token_dec Layer1.Crash o1) then
+        o2 = {| token_list := [Crash]; refinement_length := length o1 |}
+      else
+        o2 = {| token_list := [Cont]; refinement_length := length o1 |}
     end.
 
   Definition refines_to d1 d2 :=
-    rep d2 d1.
+    exists F, (F * rep d2)%pred d1.
 
-  Definition compiles_to T p2 p1 :=
+  Definition compilation_of T p1 p2 :=
     p1 = @compile T p2.
 
-  Definition low := Build_LTS Layer1.token Layer1.state Layer1.prog Layer1.exec.
+  Definition low := Build_LTS (list Layer1.token) Layer1.state Layer1.prog Layer1.exec.
 
-  Definition high := Build_LTS Layer2.token Layer2.state Layer2.prog Layer2.exec.
+  Definition high := Build_LTS Layer2.oracle Layer2.state Layer2.prog Layer2.exec.
 
+  Lemma star_split:
+    forall (AT : Type) (AEQ : EqDec AT) (V : Type)
+      (p q : @pred AT AEQ V) (m : @mem AT AEQ V),
+      (p * q)%pred m ->
+      exists m1 m2, mem_disjoint m1 m2 /\ p m1 /\ q m2 /\ mem_union m1 m2 = m.
+  Proof.
+    intros; unfold sep_star in *; rewrite sep_star_is in *;
+      destruct H; cleanup; eauto.
+    do 2 eexists; intuition eauto.
+  Qed.
+  
   Lemma rep_eq:
-    forall d s1 s2,
-      rep s1 d ->
-      rep s2 d ->
+    forall d s1 s2 F F',
+      (F * rep s1)%pred d ->
+      (F' * rep s2)%pred d ->
       s1 = s2.
   Proof.
     intros.
     extensionality k.
-    unfold rep in *.
-    destruct_lift H. destruct_lift H0.
-    eapply_fresh ptsto_valid in H.
-    eapply_fresh ptsto_valid in H0; cleanup.
-    destruct_fresh (nth k (bits (value_to_bits dummy2)) 0).
-    rewrite H4, H6; eauto.
-    destruct (value_to_bits dummy2); simpl in *.
+    apply star_split in H;
+      apply star_split in H0; cleanup.
+    unfold rep in *; simpl in *.
+    
+    destruct_lift H2. destruct_lift H5.
+    eapply_fresh ptsto_valid in H2.
+    eapply_fresh ptsto_valid in H5; cleanup.
+    eapply mem_union_addr in Hx; eauto.
+    eapply mem_union_addr in Hx0; eauto.
+    all: try solve [apply mem_disjoint_comm; eauto].
+    rewrite mem_union_comm in Hx, Hx0; eauto.
+    all: try solve [apply mem_disjoint_comm; eauto].
+    unfold set in *; simpl in *.
+    rewrite H3 in Hx; cleanup.
+                             
+    destruct_fresh (nth k (bits (value_to_bits dummy)) 0).
+    rewrite H9, H11; eauto.
+    
+    destruct (value_to_bits dummy); simpl in *.
     unfold valid_bitlist in *; cleanup.
     destruct (nth_in_or_default k bits 0); [|cleanup; omega].
-    apply H2 in i; cleanup.
+    apply H7 in i; cleanup.
     destruct n; cleanup; try omega.
-    specialize (H3 _ D).
-    specialize (H5 _ D); cleanup; eauto.
+    specialize (H8 _ D).
+    specialize (H10 _ D); cleanup; eauto.
+    eapply mem_union_addr in H8; eauto.
+    eapply mem_union_addr in H10; eauto.
+    all: try solve [apply mem_disjoint_comm; eauto].
+    rewrite mem_union_comm in H8, H10; eauto.
+    all: try solve [apply mem_disjoint_comm; eauto].
+    unfold set in *; simpl in *.
+    rewrite H3 in H8; cleanup; eauto.    
+  Qed.      
+
+  (*
+  Lemma oracle_refinement_deterministic:
+    forall T p2 ol1 ol2 oh sl1 sl2 p1 sl1' sl2', (* sh1 sh2 sh1' sh2' ,
+      refines_to sl1 sh1 ->
+      refines_to sl2 sh2 ->
+      *)
+      compilation_of T p1 p2 ->
+      Layer1.exec ol1 sl1 p1 sl1' ->
+      Layer1.exec ol2 sl2 p1 sl2' ->
+      result_same sl1' sl2' ->
+      (forall def, extract_ret def sl1' = extract_ret def sl2') ->
+      (*
+      Layer2.exec oh sh1 p2 sh1' ->
+      Layer2.exec oh sh2 p2 sh2' ->
+      result_same sl1' sh1' ->
+      result_same sl2' sh2' ->
+      result_same sh1' sh2' ->
+                                *)
+      oracle_refines_to T sl1 p2 ol1 oh ->
+      oracle_refines_to T sl2 p2 ol2 oh ->
+      ol1 = ol2.
+  Proof.
+    unfold compilation_of; induction p2; simpl; intros.
+    - (* Read *)
+      cleanup.
+      + (* Crashed *)
+        admit.
+      + (* Finished *)
+        clear D D0 H0 H1 H4.
+        generalize dependent ol2.
+        induction ol1; destruct ol2; simpl in *; intros; eauto; try omega.
+        intuition; cleanup.
+        destruct a0, t; try tauto.
+        erewrite H1; eauto.
+    - (* Write *)
+        cleanup.
+      + (* Crashed *)
+        admit.
+      + (* Finished *)
+        clear D D0 H0 H1 H4.
+        generalize dependent ol2.
+        induction ol1; destruct ol2; simpl in *; intros; eauto; try omega.
+        intuition; cleanup.
+        destruct a0, t; try tauto.
+        erewrite H1; eauto.
+    - (* Alloc *)
+      destruct (in_dec token_dec Layer1.Crash ol1), (in_dec token_dec Layer1.Crash ol2);
+        try solve [cleanup; tauto].
+      cleanup.
+      + (* Crashed *)
+        admit.
+      + destruct H4, H5.
+        clear H0 H1 H6 H7; cleanup.
+        clear H4.
+        generalize dependent ol2.
+        induction ol1; destruct ol2; simpl in *; intros; eauto; try omega.
+        intuition; cleanup.
+        destruct a, t; try tauto.
+        erewrite H1; eauto.
+    - (* Free *)
+      cleanup.
+      + (* Crashed *)
+        admit.
+      + (* Finished *)
+        clear D D0 H0 H1 H4.
+        generalize dependent ol2.
+        induction ol1; destruct ol2; simpl in *; intros; eauto; try omega.
+        intuition; cleanup.
+        destruct a0, t; try tauto.
+        erewrite H1; eauto.
+    - (* Ret *)
+      cleanup.
+      + (* Crashed *)
+        admit.
+      + (* Finished *)
+        clear D D0 H0 H1 H4.
+        generalize dependent ol2.
+        induction ol1; destruct ol2; simpl in *; intros; eauto; try omega.
+        intuition; cleanup.
+        destruct a, t0; try tauto.
+        erewrite H1; eauto.
+    - (* Bind *)
+      cleanup.
+      invert_exec; invert_exec; try tauto.
+      + (* Both Finished *)
+        specialize (H8 x1).
+        specialize (H7 x5).
+        cleanup.
+        edestruct H10; eauto; cleanup.
+        edestruct H11; eauto; cleanup.
+        specialize IHp2 with (2:= H0)(3:=H2); simpl in *.
+        edestruct IHp2; eauto.
+        specialize H with (2:= H1)(3:=H9); simpl in *.
+        
+      destruct oh; simpl in *.
+        cleanup; try tauto.
+        unfold refines_to in *; cleanup.
+        eapply read_ok in H; cleanup.
+        split_ors; destruct_lifts; cleanup.
+        edestruct H4.
+        
+        split_ors; cleanup.
+        
+        edestruct read_ok.
+        pred_apply' H; cancel.
+        eassign
+   *)
+
+  Axiom finished_crash_not_in :
+    forall T o s (p: Layer1.prog T) s' r,
+      Layer1.exec o s p (Finished s' r) ->
+      ~ In Layer1.Crash o.
+
+  Axiom crashed_crash_in :
+    forall T o s (p: Layer1.prog T) s',
+      Layer1.exec o s p (Crashed s') ->
+      In Layer1.Crash o.
+
+  Axiom layer1_exec_deterministic :
+    forall T o s (p: Layer1.prog T) s' s'',
+      Layer1.exec o s p s' ->
+      Layer1.exec o s p s'' ->
+      s' = s''.
+
+  Lemma exec_low_to_high_oracle:
+    forall T p2 p1 ol sl sl',
+      Layer1.exec ol sl p1 sl' ->
+      (forall d, sl' <> Failed d) ->
+      compilation_of T p1 p2 ->
+      exists oh, oracle_refines_to T sl p2 ol oh.
+  Proof.
+    unfold compilation_of;
+      induction p2; simpl; intros; cleanup;
+      try solve [ exists (match sl' with
+         | Crashed _ => {| token_list:= [Crash]; refinement_length := length ol |}
+         | Finished _ _ => {| token_list:= [Cont]; refinement_length := length ol |}
+         | Failed _ => {| token_list:= []; refinement_length := length ol |}
+         end); intros;
+        destruct sl'; simpl in *; [
+      eapply finished_crash_not_in in H;
+        destruct (in_dec token_dec Layer1.Crash ol); intuition tauto |
+      eapply crashed_crash_in in H;
+      destruct (in_dec token_dec Layer1.Crash ol); intuition tauto |
+      exfalso; eapply H0; eauto] ].
+
+    - (* Alloc *)
+      exists (match sl' with
+         | Crashed _ => {| token_list:= [Crash]; refinement_length := length ol |}
+         | Finished _ r =>
+           match r with
+           | Some a => {| token_list:= [BlockNum a]; refinement_length := length ol |}
+           | None => {| token_list:= [DiskFull]; refinement_length := length ol |}
+           end
+         | Failed _ => {| token_list:= []; refinement_length := length ol |}
+         end); intros.
+      destruct sl'; simpl in *.
+      eapply finished_crash_not_in in H;
+        destruct (in_dec token_dec Layer1.Crash ol); try intuition tauto.
+      (* XXX: We need to know about the behavior of alloc here *)
+      admit.
+      eapply crashed_crash_in in H;
+        destruct (in_dec token_dec Layer1.Crash ol); intuition tauto.
+      exfalso; eapply H0; eauto.
+      
+    - (* Bind *)
+      invert_exec; cleanup.      
+      + (* Finished *)
+        edestruct IHp2; eauto.
+        intros d Hx; inversion Hx.
+        edestruct H; eauto.
+        exists ({| token_list:= token_list x3 ++ token_list x4; refinement_length := refinement_length x3 + refinement_length x4 |}), x1.
+        right; intros.
+        do 6 eexists; intuition eauto.
+      + (* Crashed *)
+        split_ors; cleanup.
+        * edestruct IHp2; eauto.
+          intros d Hx; inversion Hx.
+        * edestruct IHp2; eauto.
+          intros d Hx; inversion Hx.
+          edestruct H; eauto.
+          do 2 eexists; right; intros.
+          do 6 eexists; intuition eauto.
+      + (* Failed *)
+        exfalso; eapply H1; eauto.
+  Abort.
+
+(*
+  Lemma exec_high_to_low_oracle:
+    forall T p2 oh sl sh sh',
+      refines_to sl sh ->
+      Layer2.exec oh sh p2 sh' ->
+      exists ol, oracle_refines_to T sl p2 ol oh.
+  Proof.
+    induction p2; simpl; intros.
+    - (* Read *)
+      inversion H0; cleanup.
+      eexists; intros.
+      
+      + (* Finished *)
+        unfold refines_to in *; cleanup.
+        eapply read_ok in H; cleanup.
+        split_ors; destruct_lifts; cleanup.
+        edestruct H4.
+        
+        split_ors; cleanup.
+        
+        edestruct read_ok.
+        pred_apply' H; cancel.
+      
+Abort.
+*)
+
+  (* XXX: We need oracle lengths to extract oracle equalities *) 
+  Axiom layer1_exec_finished_then_oracle_length_eq :
+    forall T (p: Layer1.prog T) s o1 o2 s'1 s'2 r1 r2,
+      Layer1.exec o1 s p (Finished s'1 r1) ->
+      Layer1.exec o2 s p (Finished s'2 r2) ->
+      length o1 = length o2.
+
+  Lemma app_split_length_eq :
+    forall T (l1 l2 l1' l2': list T),
+      l1++l2 = l1'++l2' ->
+      length l1 = length l1' ->
+      l1 = l1' /\ l2 = l2'.
+  Proof.
+    induction l1; simpl; intros.
+    symmetry in H0.
+    apply length_zero_iff_nil in H0; cleanup.
+    simpl; eauto.
+
+    destruct l1'; simpl in *.
+    inversion H0.
+    cleanup.
+    edestruct IHl1; eauto; cleanup; eauto.
   Qed.
-  
+    
   Theorem sbs :
-    forall valid_h valid_op_h,
+    forall valid_h valid_prog_h,
     StrongBisimulation low high
                        (refines_to_valid refines_to valid_h)
-                       (compiles_to_valid valid_op_h compiles_to)
+                       (compiles_to_valid valid_prog_h compilation_of)
                        valid_h
-                       valid_op_h
-                       compiles_to refines_to
-                       oracle_matches.
+                       valid_prog_h
+                       compilation_of refines_to
+                       oracle_refines_to.
+                      
   Proof.
-    unfold refines_to_valid, refines_to,
-    compiles_to_valid, compiles_to, oracle_matches; intros.
     constructor.
     intros T p1 p2.
     generalize dependent p1.
     induction p2; intros.
-    - (* Read *)
-      simpl in *; cleanup.
+    { (* Read *)
+      unfold refines_to_valid, refines_to,
+      compiles_to_valid, compilation_of, oracle_refines_to in *; intros.
+      simpl in *;
       split.
       + (* Low to High *)
-        intros.
-        eapply_fresh read_ok in H0.
-        2: instantiate (2:= emp); pred_apply; cancel.
-        split_ors; cleanup.
-        * (* Finished *)
-          destruct_lifts.
-          specialize (H5 x0); cleanup.
-          eexists.
-          split.
-          econstructor; eauto.
-          simpl in *.
-          repeat split; eauto.
-          intuition (cleanup; eauto).
-          unfold rep in *.
-          destruct_lift H7.
-          erewrite H13; eauto; simpl.
-          apply nth_overflow; simpl.
-          destruct (value_to_bits dummy); simpl.
-          unfold valid_bitlist in *; cleanup; eauto.
-          intros.
-          erewrite rep_eq; eauto.
-
+        intros; cleanup.
         * (* Crashed *)
-          destruct_lifts.
-          specialize (H5 x0); cleanup.
-          eexists.
-          split.
-          eapply ExecOpCrash; eauto.
-          intros; intuition.
-          inversion H9.
-          simpl in *.
-          repeat split; eauto.
-          intuition (cleanup; eauto).
-          erewrite rep_eq; eauto.
+          rewrite H4 in *.
+          eapply_fresh (read_ok a) in H3; cleanup.
+          eapply_fresh layer1_exec_deterministic in H6; eauto; cleanup.        
+          split_ors; cleanup.
+          --
+            destruct_lifts.
+            tauto.
+          --
+            destruct_lifts.
+            eexists; split.
+            eapply ExecOpCrash; eauto.
+            intros T p1 p2 Hx; inversion Hx.
+            simpl in *.
+            repeat split; eauto.
+            intuition (cleanup; eauto).
+            eapply_fresh rep_eq in H0; eauto; cleanup; eauto.
+        * (* Finished *)
+          rewrite H4 in *.
+          eapply_fresh (read_ok a) in H3; cleanup.
+          eapply_fresh layer1_exec_deterministic in H6; eauto; cleanup.        
+          split_ors; cleanup.
+          --
+            destruct_lifts.
+            eexists; split.
+            econstructor; eauto.
+            simpl in *.
+            repeat split; eauto.
+            
+            intuition (cleanup; eauto).
+            apply star_split in H0; cleanup.
+            unfold rep in *.
+            destruct_lift H9.          
+            erewrite H13; eauto; simpl.
+            apply nth_overflow; simpl.
+            destruct (value_to_bits dummy); simpl.
+            unfold valid_bitlist in *; cleanup; eauto.
+            
+            intros; cleanup.
+            eapply_fresh rep_eq in H0; eauto; cleanup; eauto.
+          --
+            destruct_lifts.
+            exfalso; eauto.
 
       + (*High to low*)
-        intros.
-        inversion H0; sigT_eq.
-        (* Total correctness needed 
-           to show that such execution exists *)
+        intros; cleanup.
+        * (* Crashed *)
+        eapply (read_ok a) in H3; cleanup.
+        split_ors; cleanup.
+        --
+          destruct_lifts.
+          exfalso; eauto.
+        --
+          destruct_lifts.
+          inversion H6; sigT_eq; simpl in *; cleanup.
+          eexists; split.
+          eauto.
+          simpl in *.
+          repeat split; eauto.
+          intuition (cleanup; eauto).
+          eapply_fresh rep_eq in H3; eauto;
+            cleanup; eauto.
+          
+        * (* Finished *)
+          eapply (read_ok a) in H3; cleanup.
+          split_ors; cleanup.
+          --
+            destruct_lifts.
+            inversion H6; sigT_eq; simpl in *; cleanup.
+            eexists; split.
+            eauto.
+            simpl in *.
+            repeat split; eauto.
+
+            intuition (cleanup; eauto).
+            apply star_split in H3; cleanup.
+            unfold rep in *.
+            destruct_lift H9.          
+            erewrite H13; eauto; simpl.
+            apply nth_overflow; simpl.
+            destruct (value_to_bits dummy); simpl.
+            unfold valid_bitlist in *; cleanup; eauto.
+          
+            intros; cleanup.
+            eapply_fresh rep_eq in H3; eauto;
+              cleanup; eauto.
+          --
+            destruct_lifts.
+            exfalso; eauto.
+    }
+    { (* Write *) 
+      admit.
+    }
+    { (* Alloc *)
+      admit.
+    }
+    { (* Free *)
+      admit.
+    }
+    { (* Ret *)
+      admit.
+    }
+    { (* Bind *)
+      unfold compilation_of in *; simpl in *; cleanup.
+      split; intros.
+      - (* Low to High *)
+        invert_exec.
+        + (* Finished *)
+          split_ors; cleanup.
+          * (* XXX: If Finished with o, then cannot crash with o++o' *)
+            admit.
+          *            
+            eapply_fresh layer1_exec_finished_then_oracle_length_eq in H8; eauto.
+            apply app_split_length_eq in H6; eauto; cleanup.
+            eapply_fresh layer1_exec_deterministic in H8; eauto; cleanup.
+            eapply_fresh layer1_exec_deterministic in H9; eauto; cleanup.
+          
+            edestruct IHp2; eauto.
+            unfold compiles_to_valid;
+            eexists; split; eauto.
+            (* XXX: If bind is valid, then parts are valid too *)
+            admit.
+            admit.
+            edestruct H5; eauto; simpl in *; cleanup; try tauto.
+            clear H5 H6.
+            simpl in *.
+            destruct H14; eauto; cleanup.
+            
+            edestruct H; try reflexivity; eauto.
+            unfold compiles_to_valid;
+            eexists; split; eauto.
+            (* XXX: If bind is valid, then parts are valid too *)
+            admit.
+            admit.
+            edestruct H5; eauto; simpl in *; cleanup; try tauto.
+            clear H5 H6.
+            simpl in *.
+            destruct H19; eauto; cleanup.
+            
+            eexists; split.
+            econstructor; eauto.
+            
+            simpl in *.
+            intuition eauto.
+        + (* Crashed *)
+          destruct H5; cleanup.
+          * (* First Crashed *)
+            split_ors; cleanup.
+            --
+              edestruct IHp2; eauto.
+              unfold compiles_to_valid;
+              eexists; split; eauto.
+              (* XXX: If bind is valid, then parts are valid too *)
+              admit.
+              admit.
+              edestruct H8; eauto; simpl in *; cleanup; try tauto.
+              clear H8 H9.
+              simpl in *.
+              
+              eexists; split.
+              eapply ExecBindCrash; eauto.
+              simpl in *; intuition eauto.
+            -- (* XXX: If Finished with o, then cannot crash with o++o' *)
+              admit.
+          * (* Second Crashed *)
+             split_ors; cleanup.
+             -- (* XXX: If Finished with o, then cannot crash with o++o' *)
+              admit.
+             --
+               eapply_fresh layer1_exec_finished_then_oracle_length_eq in H8; eauto.
+               apply app_split_length_eq in H6; eauto; cleanup.
+               eapply_fresh layer1_exec_deterministic in H8; eauto; cleanup.
+               eapply_fresh layer1_exec_deterministic in H9; eauto; cleanup.
+               
+               edestruct IHp2; eauto.
+               unfold compiles_to_valid;
+               eexists; split; eauto.
+               (* XXX: If bind is valid, then parts are valid too *)
+               admit.
+               admit.
+               edestruct H5; eauto; simpl in *; cleanup; try tauto.
+               clear H5 H6.
+               simpl in *.
+               destruct H14; eauto; cleanup.
+            
+               edestruct H; try reflexivity; eauto.
+               unfold compiles_to_valid;
+               eexists; split; eauto.
+               (* XXX: If bind is valid, then parts are valid too *)
+               admit.
+               admit.
+               edestruct H5; eauto; simpl in *; cleanup; try tauto.
+               clear H5 H6.
+               simpl in *.
+               
+               eexists; split.
+               econstructor; eauto.
+               
+               simpl in *.
+               intuition eauto.
+        + (* Failed *)
+          destruct H5; cleanup.
+          * (* First Failed *)
+            split_ors; cleanup.
+            --
+              eapply layer1_exec_deterministic in H6;
+              eauto; inversion H6.
+            -- (* XXX: If Finished with o, then cannot crash with o++o' *)
+              admit.
+          * (* Second Failed *)
+            split_ors; cleanup.
+            -- (* XXX: If Finished with o, then cannot crash with o++o' *)
+              admit.
+            --
+              eapply_fresh layer1_exec_finished_then_oracle_length_eq in H8; eauto.
+              apply app_split_length_eq in H6; eauto; cleanup.
+              eapply_fresh layer1_exec_deterministic in H8; eauto; cleanup.
+              eapply_fresh layer1_exec_deterministic in H9; eauto; cleanup.
+
+            edestruct IHp2; eauto.
+            unfold compiles_to_valid;
+            eexists; split; eauto.
+            (* XXX: If bind is valid, then parts are valid too *)
+            admit.
+            admit.
+            edestruct H5; eauto; simpl in *; cleanup; try tauto.
+            clear H5 H6.
+            simpl in *.
+            destruct H14; eauto; cleanup.
+            
+            edestruct H; try reflexivity; eauto.
+            unfold compiles_to_valid;
+            eexists; split; eauto.
+            (* XXX: If bind is valid, then parts are valid too *)
+            admit.
+            admit.
+            edestruct H5; eauto; simpl in *; cleanup; try tauto.
+            clear H5 H6.
+            simpl in *.
+            
+            eexists; split.
+            econstructor; eauto.
+            
+            simpl in *.
+            intuition eauto.
+            
+      - (* High to Low *)
+        unfold compiles_to_valid in H1; cleanup.
+        inversion H5; sigT_eq; clear H5.
+        + (* Finished *)
+          split_ors; cleanup.
+          (* XXX: HERE *)
   Abort.
 
 End Layer1to2Refinement.
