src/SimulationLayer.v
@@ -2,10 +2,10 @@ Require Import List CommonAutomation Simulation.
 
 Record LTS :=
   {
-    Token : Type;
+    Oracle : Type;
     State : Type;
     Prog : Type -> Type;
-    exec : forall T, list Token -> State -> Prog T -> @Result State T -> Prop;
+    exec : forall T, Oracle -> State -> Prog T -> @Result State T -> Prop;
   }.
 
 
@@ -68,7 +68,230 @@ Definition compiles_to_valid {Prog_L Prog_H: Type -> Type}
     compilation_of T pl ph /\
     valid_prog_h T ph.
 
+Definition oracle_refines_to_valid
+           {State1 State2 Oracle1 Oracle2: Type} {Op1 Op2: Type -> Type}
+           (oracle_refines_to: forall T, State1 -> Op2 T -> Oracle1 -> Oracle2 -> Prop)
+           (refines_to: State1 -> State2 -> Prop)
+           (compilation_of: forall T, Op1 T -> Op2 T -> Prop)
+           (valid_oracle2: forall T, Oracle2 -> State2 -> Op2 T -> Prop)
+           T (o1: Oracle1) (st1: State1) (p1: Op1 T) :=
+  forall st2 p2,
+    refines_to st1 st2 ->
+    compilation_of T p1 p2 ->
+    exists o2, oracle_refines_to T st1 p2 o1 o2 /\
+    valid_oracle2 T o2 st2 p2.
 
+Record SelfSimulation (lts: LTS)
+       (valid_state: State lts -> Prop)
+       (valid_op: forall T, Prog lts T -> Prop)
+       (R: State lts -> State lts -> Prop) :=
+  {
+    self_simulation_correct:
+      forall T o p s1 s1' s2,
+        valid_state s1 ->
+        valid_state s2 ->
+        valid_op T p ->
+        (exec lts) T o s1 p s1' ->
+        R s1 s2 ->
+        exists s2',
+          (exec lts) T o s2 p s2' /\
+          result_same s1' s2' /\
+          R (extract_state s1') (extract_state s2') /\
+          (forall def, extract_ret def s1' = extract_ret def s2') /\
+          valid_state (extract_state s1') /\
+          valid_state (extract_state s2') ;
+  }.
+
+Record StrongBisimulation
+       (lts1 lts2 : LTS)
+       (valid_state1 : State lts1 -> Prop)
+       (valid_prog1: forall T, Prog lts1 T -> Prop)
+       (valid_state2 : State lts2 -> Prop)
+       (valid_prog2: forall T, Prog lts2 T -> Prop)
+       (compilation_of: forall T, Prog lts1 T -> Prog lts2 T -> Prop)
+       (refines_to: State lts1 -> State lts2 -> Prop)
+       (oracle_refines_to: forall T, State lts1 -> Prog lts2 T -> Oracle lts1 -> Oracle lts2 -> Prop)
+  :=
+  {
+    strong_bisimulation_correct:
+      (forall T p1 p2 s1 s2 o1 o2,
+          valid_state1 s1 ->
+          valid_prog1 T p1 ->
+          
+          valid_state2 s2 ->
+          valid_prog2 T p2 ->
+          
+          refines_to s1 s2 ->
+          compilation_of T p1 p2 ->
+          oracle_refines_to T s1 p2 o1 o2 ->
+          
+          (forall s1',
+              (exec lts1) T o1 s1 p1 s1' ->
+              exists s2',
+                (exec lts2) T o2 s2 p2 s2' /\
+                result_same s1' s2' /\
+                refines_to (extract_state s1') (extract_state s2') /\
+                (forall def, extract_ret def s1' = extract_ret def s2') /\
+                valid_state1 (extract_state s1') /\ valid_state2 (extract_state s2')) /\
+          (forall s2',
+              (exec lts2) T o2 s2 p2 s2' ->
+              exists s1',
+                (exec lts1) T o1 s1 p1 s1' /\
+                result_same s1' s2' /\
+                refines_to (extract_state s1') (extract_state s2') /\
+                (forall def, extract_ret def s1' = extract_ret def s2')/\
+                valid_state1 (extract_state s1') /\ valid_state2 (extract_state s2')))
+  }.
+
+Theorem transfer_high_to_low :
+  forall low high
+
+    related_states_h
+    refines_to
+    compilation_of
+    oracle_refines_to
+
+    valid_state_h
+    valid_prog_h,
+    
+    SelfSimulation
+      high
+      valid_state_h
+      valid_prog_h
+      related_states_h ->
+    
+    StrongBisimulation
+      low
+      high
+      (refines_to_valid
+         refines_to
+         valid_state_h)
+      (compiles_to_valid
+         valid_prog_h
+         compilation_of)
+      valid_state_h
+      valid_prog_h
+      compilation_of
+      refines_to
+      oracle_refines_to ->
+    
+    SelfSimulation
+      low
+      (refines_to_valid
+         refines_to
+         valid_state_h)
+      (compiles_to_valid
+         valid_prog_h
+         compilation_of)
+      (refines_to_related
+         refines_to
+         related_states_h).
+Proof.
+  unfold refines_to_related, compiles_to_valid, oracle_refines_to_valid; intros.
+  destruct H, H0.
+  rename self_simulation_correct0 into self_simulation_correct.
+  rename strong_bisimulation_correct0 into strong_bisimulation_correct.
+  
+  eapply Build_SelfSimulation;  intros; cleanup.
+
+  (* PROBLEM: this requires for us to know that low oracle refines to some high oracle for s1 *)
+  (* SUGGESTION : exec low -> existence of high oracle *)
+  assume (Axiom1 : (forall T o1 s1 s1' p1 p2,
+             exec low T o1 s1 p1 s1' ->
+             compilation_of T p1 p2 ->
+             exists o2, oracle_refines_to T s1 p2 o1 o2)).
+  edestruct Axiom1; eauto.
+  (*
+  match goal with
+  | [H: refines_to ?s _,
+     H0: compilation_of _ ?p _,
+     H1: forall _ _,
+       refines_to ?s _ ->
+       compilation_of _ ?p _ -> _ |- _] =>
+    specialize H1 with (1:=H)(2:=H0); cleanup
+  end.  
+  *)
+  
+  match goal with
+  | [H: refines_to s1 _ |- _] =>
+    eapply_fresh strong_bisimulation_correct in H; eauto; cleanup
+  end.
+
+  match goal with
+    | [H: forall _, exec low _ _ _ _ _ -> _,
+       H0: exec low _ _ _ _ _,
+       H1: forall _, exec high _ _ _ _ _ -> _ |- _] =>
+      eapply_fresh  H in H0; cleanup; clear H H1
+  end.
+
+  match goal with
+  | [H: refines_to_valid _ _ ?s,
+     H0: refines_to ?s _,
+     H1: refines_to_valid _ _ ?t,
+     H2: refines_to ?t _ |- _] =>
+    eapply_fresh H in H0;
+      eapply_fresh H1 in H2; cleanup
+  end.
+
+  match goal with
+    | [H: exec high _ _ _ _ _ |- _] =>
+      eapply_fresh self_simulation_correct in H; eauto; cleanup
+  end.
+
+  (* PROBLEM: this requires for us to know that low oracle refines to some high oracle for s2 *)
+  (* SUGGESTION : exec high -> existence of low oracle *)
+  assume (Axiom2 : (forall T o2 s2 s2' l2 p2,
+             exec high T o2 s2 p2 s2' ->
+             refines_to l2 s2 ->
+             exists o1, oracle_refines_to T l2 p2 o1 o2)).
+  edestruct Axiom2; eauto.
+  
+  match goal with
+  | [H: exec high _ _ ?x2 _ _,
+     H0: refines_to ?s1 ?x1,
+     H1: refines_to ?s2 ?x2,      
+     H2: refines_to_valid _ _ ?s2 |- _] =>
+      eapply_fresh strong_bisimulation_correct in H1; eauto; cleanup
+  end.
+  
+  match goal with
+    | [H: forall _, exec low _ _ _ _ _ -> _,
+       H0: exec high _ _ _ _ _,
+       H1: forall _, exec high _ _ _ _ _ -> _ |- _] =>
+      eapply_fresh H1 in H0; cleanup; clear H H1
+  end.
+
+  (* PROBLEM: two low oracles need to be the same *)
+  (* SUGGESTION : oracle refinement is deterministic *)
+  assume (Axiom3 : (forall T ol1 ol2 oh s1 s2 p2,
+             oracle_refines_to T s1 p2 ol1 oh ->
+             oracle_refines_to T s2 p2 ol2 oh ->
+             ol1 = ol2)).
+  
+  match goal with
+    | [H: oracle_refines_to _ _ _ _ _,
+       H0: oracle_refines_to _ _ _ _ _ |- _] =>
+      specialize Axiom3 with (1:=H)(2:=H0); cleanup
+  end.
+  
+  
+  do 2 eexists; intuition eauto.
+  do 2 (eapply result_same_transitive; eauto).
+  apply result_same_symmetric; auto.
+  
+  repeat match goal with
+  | [H: forall _, extract_ret _ ?a = _ |- extract_ret _ ?a = _] =>
+    rewrite H; auto
+  end.
+Abort.
+
+
+
+
+
+
+
+(*
 Definition oracle_refines_to_valid
            {State1 State2 Oracle1 Oracle2: Type} {Op1 Op2: Type -> Type}
            (oracle_refines_to: forall T, State1 -> Op2 T -> Oracle1 -> Oracle2 -> Prop)
@@ -287,3 +510,4 @@ Proof.
     rewrite H; auto
   end.
 Qed.
+*)
